src/tls/Model.AEAD.fst
@@ -29,7 +29,7 @@ let table
 noeq
 type state (a: SC.supported_alg) (phi: plain_pred) = {
   kv: SC.kv a;
-  table: (if F.ideal_AEAD then table a kv phi else unit)
+  table: (if F.ideal_iv then table a kv phi else unit)
 }
 
 let state_kv
@@ -42,12 +42,12 @@ let state_table
   (#a: SC.supported_alg) (#phi: plain_pred)
   (s: state a phi)
 : Pure (table a (state_kv s) phi)
-  (requires (Flags.ideal_AEAD == true))
+  (requires (Flags.ideal_iv == true))
   (ensures (fun _ -> True))
 = s.table <: table a (state_kv s) phi
 
 let invariant (#a: SC.supported_alg) (#phi: plain_pred) (h: HS.mem) (s: state a phi) : GTot Type0 =
-  if F.ideal_AEAD
+  if F.ideal_iv
   then
     h `HS.contains` state_table s
   else
@@ -55,7 +55,7 @@ let invariant (#a: SC.supported_alg) (#phi: plain_pred) (h: HS.mem) (s: state a 
 
 let footprint
   #a #phi s
-= if F.ideal_AEAD
+= if F.ideal_iv
   then
     B.loc_mreference (state_table s)
   else
@@ -63,26 +63,37 @@ let footprint
 
 let frame_invariant
   #a #phi h s l h'
-= if F.ideal_AEAD
+= if F.ideal_iv
   then
     B.modifies_mreference_elim (state_table s) l h h' // FIXME: WHY WHY WHY do I need to call this lemma by hand?
   else
     ()
 
+let fresh_iv
+  #a #phi h s iv
+= F.ideal_iv == true ==> MDM.fresh (state_table s) iv h
+
+let frame_fresh_iv
+  #a #phi h s iv l h'
+= ()
+
+let is_fresh_iv
+  #a #phi s iv
+= None? (MDM.lookup (state_table s) iv)
+
 let encrypt
   #a #phi s iv plain
 = let cipher = SC.encrypt (state_kv s) iv Seq.empty plain in
-  if F.ideal_AEAD
+  if F.ideal_iv
   then begin
     let h = HST.get () in
     let tbl = state_table s in
-    assume (~ (MDM.defined tbl iv h)); // cryptographic assumption
     MDM.extend tbl iv (| cipher, plain |);
     let h' = HST.get () in
     B.modifies_loc_regions_intro (Set.singleton (HS.frameOf tbl)) h h' ;
     B.modifies_loc_addresses_intro (HS.frameOf tbl) (Set.singleton (HS.as_addr tbl)) B.loc_none h h' ;
     assume (HST.equal_domains h h'); // TODO: fix FStar.Monotonic.DependentMap
-    Seq.create (SC.cipher_length plain) (Crypto.Util.IntCast.to_sec8 0uy)
+    if F.ideal_AEAD then Seq.create (SC.cipher_length plain) (Crypto.Util.IntCast.to_sec8 0uy) else cipher
   end else
     cipher
 
