src/tls/Flags.fst
@@ -7,6 +7,7 @@ inline_for_extraction let ideal_Nonce = false
 inline_for_extraction let ideal_Sig = false
 inline_for_extraction let ideal_PMS = false
 inline_for_extraction let ideal_PRF = false
+inline_for_extraction let ideal_iv = false
 inline_for_extraction let ideal_AEAD = false
 inline_for_extraction let ideal_HMAC = false
 
